systems/Disk.v
@@ -7,37 +7,32 @@ Set Implicit Arguments.
 Section Disk.
   Context {orig_base_params : BaseParams}.
   Context {orig_multi_params : MultiParams orig_base_params}.
+  Context {orig_failure_params : FailureParams orig_multi_params}.
   Context {data_serializer : Serializer data}.
 
-  Definition disk := IOStreamWriter.wire.
-
-  Definition init_disk h := serialize_top serialize (init_handlers h).
+  Definition init_disk h := serialize_top serialize (reboot (init_handlers h)).
   
   Definition disk_net_handlers dst src m st :=
-    match net_handlers dst src m st with
-    | (out, data, packets) => 
-      (serialize_top serialize data, out, data, packets)
-    end.
+    let '(out, data, ps) := net_handlers dst src m st in
+    (serialize_top serialize (reboot data), out, data, ps).
 
   Definition disk_input_handlers h inp st :=
-    match input_handlers h inp st with
-    | (out, data, packets) => 
-      (serialize_top serialize data, out, data, packets)
-    end.
+    let '(out, data, ps) := input_handlers h inp st in
+    (serialize_top serialize (reboot data), out, data, ps).
 
-  Instance base_params : BaseParams :=
+  Instance disk_base_params : BaseParams :=
     {
       data := data ;
       input := input ;
       output := output
     }.
 
-  Instance disk_params : DiskParams base_params :=
+  Instance disk_multi_params : DiskMultiParams disk_base_params :=
     {
       d_name := name;
       d_name_eq_dec := name_eq_dec;
       d_msg := msg;
-      disk := disk;
+      disk := IOStreamWriter.wire;
       d_msg_eq_dec := msg_eq_dec;
       d_nodes := nodes;
       d_all_names_nodes := all_names_nodes;
@@ -48,12 +43,12 @@ Section Disk.
       d_input_handlers := disk_input_handlers
     }.
 
-  Instance disk_failure_params : DiskFailureParams disk_params :=
+  Instance disk_failure_params : DiskFailureParams disk_multi_params :=
     {
       d_reboot := deserialize_top deserialize
     }.
 End Disk.
 
-Hint Extern 5 (@BaseParams) => apply base_params : typeclass_instances.
-Hint Extern 5 (@DiskParams _) => apply disk_params : typeclass_instances.
-Hint Extern 5 (@DiskFailureParams _) => apply disk_failure_params : typeclass_instances.
+Hint Extern 5 (@BaseParams) => apply disk_base_params : typeclass_instances.
+Hint Extern 5 (@DiskMultiParams _) => apply disk_multi_params : typeclass_instances.
+Hint Extern 5 (@DiskFailureParams _ _) => apply disk_failure_params : typeclass_instances.
